WIP

concurrency/Modular/templates/bak_bst_giveup_specs.v
@@ -16,18 +16,27 @@ Definition struct_dlist := Tstruct _DList noattr.
 Definition t_struct_node := Tstruct _node_t noattr.
 Definition t_struct_nodeds := Tstruct _node noattr.
 
-Definition fst_list : list (val * val * val * val) -> list val := map (fun '(x, _, _,_) => x).
-Definition snd_list : list (val * val * val * val) -> list val := map (fun '(_, x, _,_) => x).
+Definition fst_list : list (val * val * val * val) -> list val :=
+  fun triples => map (fun '(x, _, _,_) => x) triples.
+
+Definition snd_list : list (val * val * val * val) -> list val :=
+  fun triples => map (fun '(_, x, _,_) => x) triples.
+
 Definition thrd_frth_list: list (val * val * val * val) -> list (val * val) :=
-  map (fun '(_, _, x, y) => (x, y)).
+  fun triples => map (fun '(_, _, x, y) => (x, y)) triples.
+
+
 Definition fst_snd_list: list (val * val * val * val) -> list (val * val) :=
-  map (fun '(x, y, _,_) => (x, y)).
+  fun triples => map (fun '(x, y, _,_) => (x, y)) triples.
+
 (*getting p that points to min *)
+
 Definition fst_thrd_list: list (val * val * val * val) -> list (val * val) :=
-  map (fun '(x, _, y,_) => (x, y)).
+  fun triples => map (fun '(x, _, y,_) => (x, y)) triples.
+
 (*getting p that points to max *)
 Definition fst_frth_list: list (val * val * val * val) -> list (val * val) :=
-  map (fun '(x, _, _, y) => (x, y)).
+  fun triples => map (fun '(x, _, _, y) => (x, y)) triples.
 
 Section bst_give_up.
   Context {N: NodeRep}.
@@ -50,10 +59,10 @@ Definition surely_malloc_spec :=
 
 Definition insertOp_spec :=
   DECLARE _insertOp
-    WITH x: Z, stt: Z, v: val, p: val, tp: val, l: val, dl: val, next: list val,
+    WITH x: Z, stt: Z, v: val, p: val, tp: val, l: val, dl: val, next: list val, r: node_info,
                     g: gname, gv: globals
   PRE [ tptr (tptr t_struct_nodeds), tint, tptr tvoid, tint, tptr (struct_dlist)]
-  PROP (repable_signed x; is_pointer_or_null v; length next = node_size)
+  PROP (repable_signed x; is_pointer_or_null v; key_in_range x r.1.2 = true; length next = node_size)
   PARAMS (p; Vint (Int.repr x); v; Vint (Int.repr stt); l)
   GLOBALS (gv)
   SEP (mem_mgr gv; field_at Tsh (struct_dlist) [StructField _list] dl l *
@@ -66,62 +75,92 @@ Definition insertOp_spec :=
   PROP (pnt <> nullval)
   LOCAL ()
   SEP (mem_mgr gv; data_at Ews (tptr t_struct_nodeds) pnt p;
-       node_rep_R pnt (Some (Some (x, v, next))) g;
+       node_rep_R pnt r.1.2 (Some (Some (x, v, next))) g;
        field_at Tsh struct_dlist (DOT _list) dl l;
        data_at Ews (tarray (tptr tvoid) (Zlength next)) next dl).
 
+(*
 
-Definition post_insert_giveup1 (p pnt : val) (x: Z) v
-  min max (trl : list (val * val * val * val)) g :=
-       iter_sepcon (fun pn => malloc_token Ews t_struct_node pn) (fst_list trl) * 
+Lemma test (trl : list (val * val * val * val)):
+  (iter_sepcon (fun '(pn, lk, fs, ft) =>
+                  malloc_token Ews t_struct_node pn *
+                  field_at Ews t_struct_node (DOT _t) (Vlong (Int64.repr 0)) pn *
+                  atomic_int_at Ews (vint 0) lk *
+                  field_at Ews t_struct_node (DOT _lock) lk pn *
+                  field_at Ews t_struct_node (DOT _min) fs pn *
+                  field_at Ews t_struct_node (DOT _max) ft pn) trl ) |--
+iter_sepcon (fun pn => malloc_token Ews t_struct_node pn) (fst_list trl) *
        iter_sepcon (fun pn => field_at Ews t_struct_node (DOT _t) (Vlong (Int64.repr 0)) pn)
-         (fst_list trl) * 
+         (fst_list trl) *
        iter_sepcon (fun lk => atomic_int_at Ews (vint 0) lk) (snd_list trl) * 
        iter_sepcon (fun fs => field_at Ews t_struct_node (DOT _lock) (snd fs) (fst fs))
-         (fst_snd_list trl) * 
+         (fst_snd_list trl) *
        iter_sepcon (fun ft => field_at Ews t_struct_node (DOT _min) (snd ft) (fst ft))
-         (fst_thrd_list trl) * 
+         (fst_thrd_list trl) *
        iter_sepcon (fun ff => field_at Ews t_struct_node (DOT _max) (snd ff) (fst ff))
-         (fst_frth_list trl) * 
-       node_rep_R pnt (Some (Some (x, v, (fst_list trl)))) g *
+         (fst_frth_list trl).
+Proof.
+  simpl.
+  Search iter_sepcon.
+  induction trl. simpl.
+  cancel.
+  replace (a :: trl) with ([a]++trl); auto.
+  rewrite ! iter_sepcon_app.
+  sep_apply IHtrl.
+  simpl.
+  destruct a.
+  destruct p. destruct p. simpl. entailer !.
+Qed.
+
+ *)
+
+ (* triple (pointer, lock, min, max) *)
+Definition post_insert_giveup1 (p pnt : val) (x: Z) v (rg: range)
+  min max (trl : list (val * val * val * val)) g :=
+       (iter_sepcon (fun '(pn, lk, fs, ft) =>
+                  malloc_token Ews t_struct_node pn *
+                  field_at Ews t_struct_node (DOT _t) nullval pn *
+                  atomic_int_at Ews (vint 0) lk *
+                  field_at Ews t_struct_node (DOT _lock) lk pn *
+                  field_at Ews t_struct_node (DOT _min) fs pn *
+                  field_at Ews t_struct_node (DOT _max) ft pn) trl) *
+       node_rep_R pnt rg (Some (Some (x, v, (fst_list trl)))) g *
        field_at Ews t_struct_node (DOT _t) pnt p *
        field_at Ews t_struct_node (DOT _min) (vint min) p * 
        field_at Ews t_struct_node (DOT _max) (vint max) p.
 
-Definition post_insert_giveup2 (p pnt tp: val) (x: Z) v 
-  min max (trl : list (val * val * val * val)) (r: node_info) g :=
-       iter_sepcon (fun pn => malloc_token Ews t_struct_node pn) (fst_list trl) * 
-       iter_sepcon (fun pn => field_at Ews t_struct_node (DOT _t) tp pn)
-         (fst_list trl) * 
-       iter_sepcon (fun lk => atomic_int_at Ews (vint 0) lk) (snd_list trl) * 
-       iter_sepcon (fun fs => field_at Ews t_struct_node (DOT _lock) (snd fs) (fst fs))
-         (fst_snd_list trl) * 
-       iter_sepcon (fun ft => field_at Ews t_struct_node (DOT _min) (snd ft) (fst ft))
-         (fst_thrd_list trl) * 
-       iter_sepcon (fun ff => field_at Ews t_struct_node (DOT _max) (snd ff) (fst ff))
-         (fst_frth_list trl) * 
-       node_rep_R tp r.2 g * node_rep_R pnt (Some (Some (x, v, (fst_list trl)))) g *
-       field_at Ews t_struct_node (DOT _t) pnt p * 
+(* For list, just a dummy function for BST *)
+Definition post_insert_giveup2 (p pnt : val) (x: Z) v (rg: range)
+  min max (trl : list (val * val * val * val)) g :=
+       (iter_sepcon (fun '(pn, lk, fs, ft) =>
+                  malloc_token Ews t_struct_node pn *
+                  field_at Ews t_struct_node (DOT _t) nullval pn *
+                  atomic_int_at Ews (vint 0) lk *
+                  field_at Ews t_struct_node (DOT _lock) lk pn *
+                  field_at Ews t_struct_node (DOT _min) fs pn *
+                  field_at Ews t_struct_node (DOT _max) ft pn) trl) *
+       node_rep_R pnt rg (Some (Some (x, v, (fst_list trl)))) g *
+       field_at Ews t_struct_node (DOT _t) pnt p *
        field_at Ews t_struct_node (DOT _min) (vint min) p * 
        field_at Ews t_struct_node (DOT _max) (vint max) p.
 
-(*
-node_rep_R tp r.1.2 r.2 g * field_at Ews t_struct_node (DOT _max) (vint max) p1
-  |-- field_at Ews t_struct_node (DOT _max) (vint Int.max_signed) p1
 
- *)
-(*
-Check Int.eq (Int.repr 2%Z) Int.zero. 
+
+(* For BST, stt <> 2 never happens, just want to have the same spec for all specific ds
+   since stt == 2 then tp = nullval (only for BST) *)
 Definition insertOp_giveup_spec :=
   DECLARE _insertOp_giveup
     WITH x: Z, stt: Z,  v: val, p: val, tp: val, min: Z, max: Z, r: node_info, g: gname, gv: globals
   PRE [ tptr t_struct_node, tint, tptr tvoid, tint ]
   PROP (repable_signed min; repable_signed max; repable_signed x;
-        is_pointer_or_null v; is_pointer_or_null v; is_pointer_or_null tp; key_in_range x r.1.2 = true)
+        is_pointer_or_null v; key_in_range x r.1.2 = true; tp = nullval )
   PARAMS (p; Vint (Int.repr x); v; Vint (Int.repr stt))
   GLOBALS (gv)
   SEP (mem_mgr gv;
-       !!(if (Int.eq (Int.repr stt) (Int.repr 2%Z)) then (tp = nullval) else (tp <> nullval)) && seplog.emp;
+       match (Int.eq (Int.repr stt) (Int.repr 2%Z)) with
+        | true => (!!(tp = nullval) && seplog.emp)
+        | false => (!!(tp <> nullval) && seplog.emp)
+       end;
        field_at Ews t_struct_node (DOT _t) tp p;
        field_at Ews t_struct_node (DOT _min) (vint min) p;
        field_at Ews t_struct_node (DOT _max) (vint max) p;
@@ -131,53 +170,10 @@ Definition insertOp_giveup_spec :=
   PROP (pnt <> nullval)
   LOCAL ()
   SEP (mem_mgr gv;
-       field_at Ews t_struct_node (DOT _t) pnt p;
-       (* malloc_token Ews t_struct_nodeds pnt; *)
-       iter_sepcon (fun pn => malloc_token Ews t_struct_node pn) (fst_list trl);
-       iter_sepcon (fun pn => field_at Ews t_struct_node (DOT _t) (Vlong (Int64.repr 0)) pn)
-         (fst_list trl);
-       iter_sepcon (fun lk => atomic_int_at Ews (vint 0) lk) (snd_list trl);
-       iter_sepcon (fun fs => field_at Ews t_struct_node (DOT _lock) (snd fs) (fst fs))
-         (fst_snd_list trl);
-       iter_sepcon (fun ft => field_at Ews t_struct_node (DOT _min) (snd ft) (fst ft))
-         (fst_thrd_list trl);
-       iter_sepcon (fun ff => field_at Ews t_struct_node (DOT _max) (snd ff) (fst ff))
-         (fst_frth_list trl);
-       node_rep_R pnt r.1.2 (Some (Some (x, v, (fst_list trl)))) g;
-       field_at Ews t_struct_node (DOT _min) (vint min) p;
-       field_at Ews t_struct_node (DOT _max) (vint max) p).
- *)
-Check Finite_Integer.
-Check (vint _).
-Check number2Z.
-Definition insertOp_giveup_spec :=
-  DECLARE _insertOp_giveup
-    WITH x: Z, stt: Z,  v: val, p: val, tp: val, min: Z, max: Z, r: node_info, g: gname, gv: globals
-  PRE [ tptr t_struct_node, tint, tptr tvoid, tint ]
-  PROP (repable_signed min; repable_signed max; repable_signed x;
-        is_pointer_or_null v; is_pointer_or_null v; is_pointer_or_null tp; tp = nullval)
-  PARAMS (p; Vint (Int.repr x); v; Vint (Int.repr stt))
-  GLOBALS (gv)
-  SEP (mem_mgr gv;
        match (Int.eq (Int.repr stt) (Int.repr 2%Z)) with
-        | true => (!!(tp = nullval /\ (r.2 = Some None) ) && seplog.emp)
-        | false => (!!(tp <> nullval) && seplog.emp)
-       end;
-       field_at Ews t_struct_node (DOT _t) tp p;
-       field_at Ews t_struct_node (DOT _min) (vint min) p;
-       field_at Ews t_struct_node (DOT _max) (vint max) p;
-       node_rep_R tp r.2 g )
-  POST[ tvoid ] (* triple (pointer, lock, min, max) *)
-  EX (pnt : val) (trl : list (val * val * val * val)),
-  PROP (pnt <> nullval)
-  LOCAL ()
-  SEP (mem_mgr gv;
-       (match (Int.eq (Int.repr stt) (Int.repr 2%Z)) with
-        | true => (post_insert_giveup1 p pnt x v min max trl g)
-        | _    => (post_insert_giveup2 p pnt tp x v min
-                   max trl r g)
-        end)).
-
+       | true =>  (post_insert_giveup1 p pnt x v r.1.2 min max trl g)
+       | false => (post_insert_giveup2 p pnt x v r.1.2 min max trl g)
+       end).
 
 Definition Gprog : funspecs :=
     ltac:(with_library prog [acquire_spec; release_spec; makelock_spec;  
@@ -219,9 +215,8 @@ Proof.
   unfold_data_at (data_at _ _ _ v_dlist).
   assert (field_address t_struct_node (DOT _t) p  = p) as I.
   rewrite -> field_compatible_field_address, isptr_offset_val_zero; auto.
-  Intros.
   forward_call(x, stt, v, (field_address t_struct_node  [StructField _t] p), tp,
-                v_dlist, lst, [p1; p2] , g, gv).
+                v_dlist, lst, [p1; p2] , r, g, gv).
   entailer !.
   Intros pnt.
   forward. forward. entailer !. list_solve.
@@ -243,9 +238,8 @@ Proof.
   unfold post_insert_giveup1.
   simpl.
   cancel.
-  rewrite node_null.
-  entailer !.
-Qed.
+  admit.
+Admitted.
 
 End bst_give_up.
 
