concurrency/Modular/templates/bak_bst_inst.v
@@ -1,9 +1,8 @@
 Require Import VST.concurrency.conclib.
 Require Import VST.floyd.proofauto.
 Require Import VST.atomics.general_locks.
-Require Import Coq.Sets.Ensembles.
 Require Import bst.puretree.
-Require Import bst.list.
+Require Import bst.bst.
 Require Import bst.data_struct.
 Require Import VST.atomics.verif_lock_atomic.
 Require Import VST.floyd.library.
@@ -12,35 +11,41 @@ Require Import VST.floyd.library.
 Definition Vprog : varspecs.  mk_varspecs prog. Defined.
 
 (* struct node {int key; void *value; struct tree_t *left, *right;} node;*)
-Definition t_struct_list := Tstruct _node noattr.
+Definition t_struct_tree := Tstruct _node noattr.
 (* Define for dynamic list *)
 Definition struct_dlist := Tstruct _DList noattr.
 
-#[local] Obligation Tactic := idtac.
+(* struct tree_t {node *t; lock_t *lock; int min; int max; } tree_t; *)
+(* Definition t_struct_tree_t := Tstruct _tree_t noattr. *)
+
 (* node_rep_R r.1.1.1 r.1.2 r.2 g, and r is type of node_info *)
+
+
+#[local] Obligation Tactic := idtac.
+
 #[local] Program Instance my_specific_tree_rep : NodeRep := {
-    node_rep_R := fun (tp : val) (g_info : option (option ghost_info)) g =>
-      if eq_dec tp nullval
-      then !!(g_info = Some None) && seplog.emp
-      else (EX (x : Z), EX (v next : val),
-      !!(g_info = Some (Some (x, v, [next])) /\ and (Z.le Int.min_signed x) (Z.le x Int.max_signed) /\
-       is_pointer_or_null next /\ (tc_val (tptr Tvoid) v)) &&
-       data_at Ews t_struct_list ((Vint (Int.repr x)), (v, next)) tp *
-       malloc_token Ews t_struct_list tp); node_size := 1 }.
+  node_rep_R := fun (tp : val) (r : range) (g_info : option (option ghost_info)) g =>
+  if eq_dec tp nullval
+  then !!(g_info = Some None) && seplog.emp
+  else
+  (EX (x : Z), EX (v pa pb : val),
+      !!(g_info = Some (Some (x, v, [pa; pb])) /\ and (Z.le Int.min_signed x) (Z.le x Int.max_signed) /\
+       is_pointer_or_null pa /\ is_pointer_or_null pb /\
+          (tc_val (tptr Tvoid) v) /\ key_in_range x r = true) &&
+       data_at Ews t_struct_tree ((Vint (Int.repr x)), (v, (pa, pb))) tp * 
+       malloc_token Ews t_struct_tree tp); node_size := 2}.
+(* ; node_rep_R_valid_pointer }. *)
 Next Obligation.
   simpl.
-  intros tp g_info g.
-  destruct (EqDec_val tp nullval); [ | Intros x v next]; entailer !.
+  intros tp r g_info g.
+  destruct (EqDec_val tp nullval); [ | Intros x v pa pb]; entailer !.
 Defined.
 Next Obligation.
   simpl.
-  intros tp g_info g.
-  destruct (EqDec_val tp nullval); [ | Intros x v next]; entailer !.
+  intros tp r g_info g.
+  destruct (EqDec_val tp nullval); [ | Intros x v pa pb]; entailer !.
 Defined.
-Next Obligation.
-  by intros g_info.
-Defined.
-    
+
 Definition extract_node_pn (node: node_info) : list val :=
   match node.2 with
   | Some (Some (_, _, lst)) => lst
@@ -49,17 +54,14 @@ Definition extract_node_pn (node: node_info) : list val :=
 
 (* Spec of findnext function *)
 (* FOUND = 0, NOTFOUND = 1, NULLNEXT = 2 (NULLNEXT = NULL || NEXT ) *)
-
-(* Spec of findnext function *)
-(* FOUND = 0, NOTFOUND = 1, NULLNEXT = 2 (NULLNEXT = NULL || NEXT ) *)
 Definition findnext_spec :=
   DECLARE _findNext
   WITH x: Z, p: val, n: val, n_pt : val, r: node_info,
                 g: gname, sh: share, gv: globals
-  PRE [ tptr t_struct_list, tptr (tptr tvoid), tint ]
+  PRE [ tptr t_struct_tree, tptr (tptr tvoid), tint ]
           PROP (writable_share sh(*; is_pointer_or_null pa; is_pointer_or_null pb*) )
           PARAMS (p; n; Vint (Int.repr x)) GLOBALS (gv)
-          SEP (node_rep_R r.1.1.1 r.2 g * (!!(p = r.1.1.1 /\ p <> nullval) && seplog.emp) *
+          SEP (node_rep_R r.1.1.1 r.1.2 r.2 g * (!!(p = r.1.1.1 /\ p <> nullval) && seplog.emp) *
                (* field_at sh (t_struct_tree) [StructField _t] r.1.1.1 p; *)
                data_at sh (tptr tvoid) n_pt n)
   POST [ tint ]
@@ -73,7 +75,8 @@ Definition findnext_spec :=
                | F | NF => data_at sh (tptr tvoid) n_pt n
                | NN => !!(n' ∈ extract_node_pn r) && data_at sh (tptr tvoid) next n
              end *
-               node_rep_R r.1.1.1 r.2 g) .
+               node_rep_R r.1.1.1 r.1.2 r.2 g) .
+
 
 Lemma findNext: semax_body Vprog Gprog f_findNext findnext_spec.
 Proof.
@@ -83,35 +86,38 @@ Proof.
   Intros.
   subst.
   rewrite -> if_false; eauto.
-  Intros x0 v0 next.
+  Intros x0 v0 pa pb.
   forward.
-  forward_if. 
+  forward_if. (* if (_x < _y) *)
   - forward. forward. forward.
-    Exists NN next next.
+    Exists NN pa pa.
+    entailer !.
     unfold extract_node_pn.
     rewrite H.
-    entailer !.
     apply elem_of_list_here.
-    unfold node_rep_R.
+    rewrite H.
     simpl.
     rewrite -> if_false; eauto.
-    Exists x0 v0 next.
+    Exists x0 v0 pa pb.
     entailer !.
   - forward_if.
     repeat forward.
-    Exists NF r.1.1.1 n_pt.
-    unfold node_rep_R.
+    Exists NN pb pb.
+    entailer !.
+    unfold extract_node_pn.
+    rewrite H. simpl.
+    assert([pa ; pb] = [pa] ++ [pb]) as K by auto.
+    rewrite K elem_of_app; right; apply elem_of_list_here. 
     simpl.
     rewrite -> if_false; eauto.
-    Exists x0 v0 next.
+    Exists x0 v0 pa pb.
     entailer !.
     forward.
-    Exists F r.1.1.1 n_pt.
+    Exists F r.1.1.1  n_pt.
     entailer !.
-    unfold node_rep_R.
     simpl.
     rewrite -> if_false; eauto.
-    Exists x0 v0 next.
+    Exists x0 v0 pa pb.
     entailer !.
 Qed.
 
@@ -132,38 +138,37 @@ Definition surely_malloc_spec :=
 
 Definition insertOp_spec :=
   DECLARE _insertOp
-    WITH x: Z, stt: Z, v: val, p: val, tp: val, l: val, dl: val, next: list val, rng: range,
+    WITH x: Z, stt: Z, v: val, p: val, tp: val, l: val, dl: val, next: list val, r: node_info,
                     g: gname, gv: globals
-  PRE [ tptr (tptr t_struct_list), tint, tptr tvoid, tint, tptr (struct_dlist)]
-  PROP (repable_signed x; is_pointer_or_null v; key_in_range x rng = true;
-        is_pointer_or_null (Znth 0 next);
+  PRE [ tptr (tptr t_struct_tree), tint, tptr tvoid, tint, tptr (struct_dlist)]
+  PROP (repable_signed x; is_pointer_or_null v; is_pointer_or_null (Znth 0 next);
+        is_pointer_or_null (Znth 1 next); key_in_range x r.1.2 = true ;
         length next = node_size)
   PARAMS (p; Vint (Int.repr x); v; Vint (Int.repr stt); l)
   GLOBALS (gv)
-  SEP (mem_mgr gv; 
-                     field_at Tsh (struct_dlist) [StructField _list] dl l *
-                     (* field_at Ews (struct_dlist) [StructField _size] (Vptrofs (Ptrofs.repr 2%Z)) l * *)
+  SEP (mem_mgr gv; field_at Ews (struct_dlist) [StructField _list] dl l *
                      data_at Ews (tarray (tptr tvoid) (Zlength next)) next dl * 
                      (* (!!(p = r.1.1.1 /\ p = nullval)  && seplog.emp); *)
-       data_at Ews (tptr t_struct_list) tp p)
+       data_at Ews (tptr t_struct_tree) tp p)
   POST[ tvoid ]
   EX (pnt : val),
   PROP (pnt <> nullval)
   LOCAL ()
-  SEP (mem_mgr gv; data_at Ews (tptr t_struct_list) pnt p;
-       node_rep_R pnt (Some (Some (x, v, next))) g;
-       field_at Tsh struct_dlist (DOT _list) dl l;
+  SEP (mem_mgr gv; data_at Ews (tptr t_struct_tree) pnt p;
+       node_rep_R pnt r.1.2 (Some (Some (x, v, next))) g;
+       field_at Ews struct_dlist (DOT _list) dl l;
        data_at Ews (tarray (tptr tvoid) (Zlength next)) next dl).
 
-Lemma length_equal_1 : forall (x: Z) (v: val) (next : list val),
-  length next = 1%nat ->
-  Some (Some (x, v, next)) = Some (Some (x, v, [Znth 0 next])).
+Lemma length_equal_2 (x: Z) (v: val) (next : list val):
+  length next = 2%nat ->
+  Some (Some (x, v, next)) = Some (Some (x, v, [Znth 0 next; Znth 1 next])).
 Proof.
-  intros x v next H_length.
+  intros H_length.
   destruct next as [|a [|b tl]] eqn:Heq_next; try discriminate.
   inversion H_length; subst.
   unfold Znth; simpl.
-  repeat f_equal.
+  repeat f_equal. 
+  by apply nil_length_inv. 
 Qed.
 
 Definition Gprog : funspecs :=
@@ -173,24 +178,30 @@ Definition Gprog : funspecs :=
 Lemma insertOp: semax_body Vprog Gprog f_insertOp insertOp_spec.
 Proof.
   start_function.
-  forward_call (t_struct_list, gv).
+  forward_call (t_struct_tree, gv).
   Intros new_node.
   forward.
   forward.
   forward.
   forward.
   entailer !.
-  simpl in H3.
-  rewrite Zlength_correct. lia.
+  simpl in H4.
+  by rewrite Zlength_correct H4.
   forward.
   forward.
-  Exists new_node .
-  assert_PROP (new_node <> nullval). entailer !.
+  forward.
+  entailer !.
+  simpl in H4.
+  by rewrite Zlength_correct H4.
+  forward.
+  forward.
+  Exists new_node.
+  assert_PROP (new_node <> nullval) by entailer !.
   unfold node_rep_R.
   unfold my_specific_tree_rep.
   rewrite if_false; auto.
   entailer !.
-  Exists x v (Znth 0 next).
+  Exists x v (Znth 0 next) (Znth 1 next).
   entailer !.
-  by apply length_equal_1.
+  by apply length_equal_2.
 Qed.
