concurrency/Modular/templates/bak_list_giveup_specs.v
@@ -49,10 +49,10 @@ Definition surely_malloc_spec :=
 
 Definition insertOp_spec :=
   DECLARE _insertOp
-    WITH x: Z, stt: Z, v: val, p: val, l: val, dl: val, next: list val,
+    WITH x: Z, stt: Z, v: val, p: val, l: val, dl: val, next: list val, rng: range,
                     g: gname, gv: globals
   PRE [ tptr (tptr t_struct_nodeds), tint, tptr tvoid, tint, tptr (struct_dlist)]
-  PROP (repable_signed x; is_pointer_or_null v;
+  PROP (repable_signed x; is_pointer_or_null v; key_in_range x rng = true;
         is_pointer_or_null (Znth 0 next);
         length next = node_size)
   PARAMS (p; Vint (Int.repr x); v; Vint (Int.repr stt); l)
@@ -68,12 +68,12 @@ Definition insertOp_spec :=
   PROP (pnt <> nullval)
   LOCAL ()
   SEP (mem_mgr gv; data_at Ews (tptr t_struct_nodeds) pnt p;
-       node_rep_R pnt (Some (Some (x, v, next))) g;
+       node_rep_R pnt rng (Some (Some (x, v, next))) g;
        field_at Tsh struct_dlist (DOT _list) dl l;
        data_at Ews (tarray (tptr tvoid) (Zlength next)) next dl).
 
 
-Definition post_insert_giveup1 (p pnt : val) (x: Z) v
+Definition post_insert_giveup1 (p pnt : val) (x: Z) v (rg: range)
   min max (trl : list (val * val * val * val)) g :=
        iter_sepcon (fun pn => malloc_token Ews t_struct_node pn) (fst_list trl) * 
        iter_sepcon (fun pn => field_at Ews t_struct_node (DOT _t) (Vlong (Int64.repr 0)) pn)
@@ -85,12 +85,12 @@ Definition post_insert_giveup1 (p pnt : val) (x: Z) v
          (fst_thrd_list trl) * 
        iter_sepcon (fun ff => field_at Ews t_struct_node (DOT _max) (snd ff) (fst ff))
          (fst_frth_list trl) * 
-       node_rep_R pnt (Some (Some (x, v, (fst_list trl)))) g *
+       node_rep_R pnt rg (Some (Some (x, v, (fst_list trl)))) g *
        field_at Ews t_struct_node (DOT _t) pnt p *
        field_at Ews t_struct_node (DOT _min) (vint min) p * 
        field_at Ews t_struct_node (DOT _max) (vint max) p.
 
-Definition post_insert_giveup2 (p pnt tp: val) (x: Z) v 
+Definition post_insert_giveup2 (p pnt tp: val) (x: Z) v (rg: range)
   min max (trl : list (val * val * val * val)) (r: node_info) g :=
        iter_sepcon (fun pn => malloc_token Ews t_struct_node pn) (fst_list trl) * 
        iter_sepcon (fun pn => field_at Ews t_struct_node (DOT _t) tp pn)
@@ -102,7 +102,7 @@ Definition post_insert_giveup2 (p pnt tp: val) (x: Z) v
          (fst_thrd_list trl) * 
        iter_sepcon (fun ff => field_at Ews t_struct_node (DOT _max) (snd ff) (fst ff))
          (fst_frth_list trl) * 
-       node_rep_R tp r.2 g * node_rep_R pnt (Some (Some (x, v, (fst_list trl)))) g *
+       node_rep_R tp rg r.2 g * node_rep_R pnt r.1.2 (Some (Some (x, v, (fst_list trl)))) g *
        field_at Ews t_struct_node (DOT _t) pnt p * 
        field_at Ews t_struct_node (DOT _min) (vint min) p * 
        field_at Ews t_struct_node (DOT _max) (vint max) p.
@@ -157,7 +157,7 @@ Definition insertOp_giveup_spec :=
     WITH x: Z, stt: Z,  v: val, p: val, tp: val, min: Z, max: Z, r: node_info, g: gname, gv: globals
   PRE [ tptr t_struct_node, tint, tptr tvoid, tint ]
   PROP (repable_signed min; repable_signed max; repable_signed x;
-        is_pointer_or_null v; is_pointer_or_null v; is_pointer_or_null tp)
+        is_pointer_or_null v; is_pointer_or_null v; is_pointer_or_null tp; key_in_range x r.1.2 = true)
   PARAMS (p; Vint (Int.repr x); v; Vint (Int.repr stt))
   GLOBALS (gv)
   SEP (mem_mgr gv;
@@ -168,15 +168,15 @@ Definition insertOp_giveup_spec :=
        field_at Ews t_struct_node (DOT _t) tp p;
        field_at Ews t_struct_node (DOT _min) (vint min) p;
        field_at Ews t_struct_node (DOT _max) (vint max) p;
-       node_rep_R tp r.2 g )
+       node_rep_R tp r.1.2 r.2 g )
   POST[ tvoid ] (* triple (pointer, lock, min, max) *)
   EX (pnt : val) (trl : list (val * val * val * val)),
   PROP (pnt <> nullval)
   LOCAL ()
   SEP (mem_mgr gv;
        (match (Int.eq (Int.repr stt) (Int.repr 2%Z)) with
-        | true => (post_insert_giveup1 p pnt x v min max trl g)
-        | _    => (post_insert_giveup2 p pnt tp x v min
+        | true => (post_insert_giveup1 p pnt x v r.1.2 min max trl g)
+        | _    => (post_insert_giveup2 p pnt tp x v (Finite_Integer x, Finite_Integer max) min
                    max trl r g)
         end)).
 
@@ -242,17 +242,17 @@ Proof.
      temp _value v; temp _status (vint stt))
      SEP ((match (Int.eq (Int.repr stt) (Int.repr 2%Z)) with
            | true => (EX (pnt: val),
-                      (!!(pnt <> nullval) && seplog.emp) * node_rep_R pnt (Some (Some (x, v, [p1]))) g * data_at Ews (tptr t_struct_nodeds) pnt (field_address t_struct_node (DOT _t) p) * data_at Ews t_struct_node (nullval , (lock, (vint x, vint Int.max_signed))) p1)
+                      (!!(pnt <> nullval) && seplog.emp) * node_rep_R pnt (Finite_Integer min, Finite_Integer max)  (Some (Some (x, v, [p1]))) g * data_at Ews (tptr t_struct_nodeds) pnt (field_address t_struct_node (DOT _t) p) * data_at Ews t_struct_node (nullval , (lock, (vint x, vint Int.max_signed))) p1)
            | false =>  (EX (pnt: val), (!!(pnt <> nullval) && seplog.emp) *
-                                        node_rep_R tp r.2 g *
-                                      node_rep_R pnt (Some (Some (x, v, [p1]))) g * data_at Ews (tptr t_struct_nodeds) pnt (field_address t_struct_node (DOT _t) p) * data_at Ews t_struct_node (tp, (lock, (vint x, vint max))) p1)
+                                        node_rep_R tp (Finite_Integer x, Finite_Integer max) r.2 g *
+                                      node_rep_R pnt (Finite_Integer min, Finite_Integer max) (Some (Some (x, v, [p1]))) g * data_at Ews (tptr t_struct_nodeds) pnt (field_address t_struct_node (DOT _t) p) * data_at Ews t_struct_node (tp, (lock, (vint x, vint max))) p1)
            end); atomic_int_at Ews (vint 0) lock; mem_mgr gv; malloc_token Ews t_struct_node p1;
      malloc_token Ews (tarray (tptr tvoid) 1) lst;
      data_at Ews (tarray (tptr tvoid) 1) [p1] lst;
      data_at Tsh (Tstruct _DList noattr) (lst, Vlong (Int64.repr (Int.signed (Int.repr 1)))) v_dlist;
      field_at Ews t_struct_node (DOT _min) (vint min) p;
      field_at Ews t_struct_node (DOT _max) (vint max) p)).
-  - rewrite H5; simpl.
+  - rewrite H6; simpl.
     Intros.
     forward. forward. forward.
     assert_PROP (field_compatible t_struct_node [] p1) by entailer!.
@@ -262,7 +262,7 @@ Proof.
     (* call insertOp *)
 
     forward_call(x, stt, v, (field_address t_struct_node [StructField _t] p), v_dlist, lst, [p1] ,
-                  g, gv).
+                  (Finite_Integer min, Finite_Integer max), g, gv).
     {
       entailer !. simpl.
       change ((((0 + Z.pos (8 * 8) - 1) `div` Z.pos (8 * 8) * Z.pos (8 * 8)) `div` 8)) with 0.
@@ -271,16 +271,17 @@ Proof.
     }
     unfold_data_at (data_at _ _ _ v_dlist).
     cancel.
-    entailer !. 
+    entailer !. Check key_in_range.
+    admit.
     Intros pnt.
     forward. forward. entailer !. list_solve.
     forward. forward. forward. entailer !. list_solve.
     forward.
-    rewrite H5.
+    rewrite H7.
     entailer !.
+    rewrite H6.
     simpl.
-    Exists pnt .
-    cancel.
+    Exists pnt . cancel.
     unfold_data_at (data_at _ _ _ v_dlist).
     entailer !.
     rewrite node_null.
@@ -296,21 +297,29 @@ Proof.
     assert (field_address t_struct_node (DOT _t) p  = p) as I.
     rewrite -> field_compatible_field_address, isptr_offset_val_zero; auto.
     forward_call(x, stt, v, (field_address t_struct_node [StructField _t] p), v_dlist, lst, [p1] ,
-                  g, gv).
+                  (Finite_Integer min, Finite_Integer max) , g, gv).
     unfold_data_at (data_at _ _ _ v_dlist).
     entailer !.
     change (Vlong (Int64.repr 0)) with nullval.
-    cancel. 
+    cancel. admit.
     rewrite Int.eq_false; auto.
     Intros pnt.
     Exists pnt.
     entailer !.
     unfold_data_at (data_at _ _ _ v_dlist).
     entailer !.
+    eapply key_node_in_range; eauto.
+    destruct r.1.2.
+    
+    Check range_incl.
+    Check less_than_equal.
+    assert (less_than_equal (Finite_Integer x) n). admit.
+    unfold range_incl.
+    
   - forward.
     assert (field_address t_struct_node (DOT _t) p = p) as I.
     {
-      clear -H5.
+      clear - H6.
       rewrite ->  field_compatible_field_address, isptr_offset_val_zero; auto.
       (* isptr p ; field_compatible t_struct_node (DOT _t) p *)
     }
@@ -348,7 +357,13 @@ Proof.
       unfold_data_at (data_at _ _ _ p1).
       unfold_data_at(data_at_ Tsh (Tstruct _DList noattr) v_dlist).
       entailer !.
+
+
+
+
+
+      
+  Admitted.
 Qed.
 
-End give_up.
 
