concurrency/Modular/templates/data_struct.v
@@ -69,10 +69,10 @@ Proof. by rewrite - bi.persistent_sep_dup. Qed.
 
 Section NodeRep.
   Class NodeRep : Type := {
-      node_rep_R : val -> range -> option (option ghost_info) -> gname -> mpred;
-      node_rep_R_valid_pointer: forall tp r g_in g, node_rep_R tp r g_in g |-- valid_pointer tp;
-      node_rep_R_pointer_null: forall tp r g_in g, node_rep_R tp r g_in g |-- !! is_pointer_or_null tp;
+      node_rep_R : val -> option (option ghost_info) -> gname -> mpred;
+      node_rep_R_valid_pointer: forall tp g_in g, node_rep_R tp g_in g |-- valid_pointer tp;
+      node_rep_R_pointer_null: forall tp g_in g, node_rep_R tp g_in g |-- !! is_pointer_or_null tp;
       node_size: nat;
-      node_null: forall r g_info, node_rep_R nullval r g_info = !!(g_info = Some None) && seplog.emp;
+      node_null: forall g_info, node_rep_R nullval g_info = !!(g_info = Some None) && seplog.emp;
   }.
 End NodeRep.
